\section{Unilinear Grammar}

A grammar is unilinear iff all rules are either all left-linear or right-linear. It can also be required that it has:
\begin{itemize}
    \item Strictly unilinear rules: $A \rarr aB$ with $a\in \Sigma \cup \epsilon$ and $B \in V \cup \epsilon$
    \item All terminal rules are empty: $B \rarr b$ replaced with $B \rarr bB'$, $B' \rarr \epsilon$
\end{itemize}

\subsection{From Unilinear to Regular Expression}

\textbf{Assumptions}: strictly right unilinear, all terminal rules empty.

For every nonterminal $A$ defined by $A \rarr a_1A_1|\ldots|a_kA_k|\epsilon$:
$L_A = a_1L_{A_1} \cup | \ldots | \cup a_kL_{A_k} \cup \epsilon$

\textbf{Arden Identity}: $X = KX \cup L$ (with $K$ nonempty) has exactly one solution $X = K^*L$.

\textbf{Example} $S \rarr sS | eA$, $A \rarr sS|\epsilon$
\begin{alignat*}{2}
&
    \begin{cases}
        L_S = sL_S \cup eL_A \\
        L_A = sL_S \cup \epsilon
    \end{cases}
&&
    \begin{cases}
        L_S = sL_S \cup e(sL_S \cup \epsilon) \\
        L_A = sL_S \cup \epsilon
    \end{cases}
\\
&
    \begin{cases}
        L_S = (s \cup es) L_S \cup e \\
        L_A = sL_S \cup \epsilon
    \end{cases}
&&
    \begin{cases}
        L_S = (s \cup es)^*e \\
        L_A = sL_S \cup \epsilon = s(s \cup es)^*e \cup \epsilon
    \end{cases}
\end{alignat*}
